upgrade mathlib

src/fin.lean
@@ -3,41 +3,60 @@ import data.equiv.fin
 
 namespace fin
 
-/-- embedding `fin n` into `fin (m + n)` sending `i` to `m + i` -/
-def cast_add_right (m : ℕ) {n : ℕ} : fin n ↪ fin (m + n) :=
-{ to_fun := λ i, ⟨m + i, add_lt_add_left i.2 _⟩,
-  inj' := λ i j h, fin.ext (by simpa using h) }
+@[elab_as_eliminator]
+def reverse_induction {n : ℕ}
+  {C : fin (n + 1) → Sort*}
+  (h0 : C (fin.last n))
+  (hs : ∀ i : fin n, C i.succ → C i.cast_succ) :
+  Π (i : fin (n + 1)), C i
+| i :=
+if hi : i = fin.last n
+then _root_.cast (by rw hi) h0
+else
+  let j : fin n :=  ⟨i, lt_of_le_of_ne (nat.le_of_lt_succ i.2) (λ h, hi (fin.ext h))⟩ in
+  have wf : n + 1 - j.succ < n + 1 - i, begin
+    cases i,
+    rw [nat.sub_lt_sub_left_iff];
+    simp [*, nat.succ_le_iff],
+  end,
+  have hi : i = fin.cast_succ j, from fin.ext rfl,
+_root_.cast (by rw hi) (hs _ (reverse_induction j.succ))
+using_well_founded { rel_tac := λ _ _, `[exact ⟨_, measure_wf (λ i : fin (n+1), n + 1 - i)⟩],
+  dec_tac := `[assumption] }
 
-@[simp] lemma coe_cast_add_right (m : ℕ) {n : ℕ} (i : fin n) :
-  (cast_add_right m i : ℕ) = m + i := rfl
+lemma reverse_induction_last {n : ℕ}
+  {C : fin (n + 1) → Sort*}
+  (h0 : C (fin.last n))
+  (hs : ∀ i : fin n, C i.succ → C i.cast_succ) :
+  (reverse_induction h0 hs (fin.last n) : C (fin.last n)) = h0 :=
+by rw [reverse_induction]; simp
 
-lemma le_cast_add_right (m : ℕ) {n : ℕ} (i : fin n) : m ≤ cast_add_right m i :=
-nat.le_add_right _ _
-
-lemma cast_add_lt {m : ℕ} (n : ℕ) (i : fin m) : (cast_add n i : ℕ) < m := i.2
+lemma reverse_induction_cast_succ {n : ℕ}
+  {C : fin (n + 1) → Sort*}
+  (h0 : C (fin.last n))
+  (hs : ∀ i : fin n, C i.succ → C i.cast_succ) (i : fin n):
+  (reverse_induction h0 hs i.cast_succ : C i.cast_succ) =
+    hs i (reverse_induction h0 hs i.succ) :=
+begin
+  rw [reverse_induction, dif_neg (ne_of_lt (fin.cast_succ_lt_last i))],
+  cases i,
+  refl
+end
 
 @[elab_as_eliminator, elab_strategy]
-def last_cases {n : ℕ} {C : fin n.succ → Sort*}
-  (hlast : C (fin.last n)) (hcast : (Π (i : fin n), C i.cast_succ)) (i : fin n.succ) : C i :=
-if hi : i = fin.last _
-then _root_.cast (by rw hi) hlast
-else have hi : i = fin.cast_succ ⟨i, lt_of_le_of_ne (nat.le_of_lt_succ i.2)
-    (λ h, hi (fin.ext h))⟩, from fin.ext rfl,
-  _root_.cast (by rw hi) (hcast _)
+def last_cases {n : ℕ} {C : fin (n + 1) → Sort*}
+  (hlast : C (fin.last n)) (hcast : (Π (i : fin n), C i.cast_succ)) (i : fin (n + 1)) : C i :=
+reverse_induction hlast (λ i _, hcast i) i
 
-@[simp] lemma last_cases_last  {n : ℕ} {C : fin n.succ → Sort*}
+@[simp] lemma last_cases_last {n : ℕ} {C : fin (n + 1) → Sort*}
   (hlast : C (fin.last n)) (hcast : (Π (i : fin n), C i.cast_succ)) :
   (fin.last_cases hlast hcast (fin.last n): C (fin.last n)) = hlast :=
-by simp [fin.last_cases]
+reverse_induction_last _ _
 
-@[simp] lemma last_cases_cast_succ  {n : ℕ} {C : fin n.succ → Sort*}
+@[simp] lemma last_cases_cast_succ {n : ℕ} {C : fin (n + 1) → Sort*}
   (hlast : C (fin.last n)) (hcast : (Π (i : fin n), C i.cast_succ)) (i : fin n) :
   (fin.last_cases hlast hcast (fin.cast_succ i): C (fin.cast_succ i)) = hcast i :=
-begin
-  simp only [fin.last_cases, dif_neg (ne_of_lt (fin.cast_succ_lt_last i)), cast_eq],
-  congr,
-  simp,
-end
+reverse_induction_cast_succ _ _ _
 
 @[elab_as_eliminator, elab_strategy]
 def add_cases {m n : ℕ} {C : fin (m + n) → Sort*}
